lawyer/nonblocking/examples/counter.v
@@ -87,7 +87,7 @@ Lemma counter_wfree_spec (l: loc)
   {M} {EM: ExecutionModel heap_lang M} {Σ : gFunctors}
     (OHE : OM_HL_Env OP_HL_WF EM Σ):
   (let _: heap1GS Σ := iem_phys HeapLangEM EM in counter_inv l)
-  ⊢ wait_free_spec_defs.wait_free_method (incr l) d_wfr0 5.
+  ⊢ wait_free_spec_defs.wait_free_method NotStuck (incr l) d_wfr0 5.
 Proof using.
   simpl. rewrite /wait_free_spec_defs.wait_free_method. 
   iIntros "#INV" (τ π q a). iIntros "!> %Φ (CPS & PH) POST".
@@ -138,7 +138,7 @@ Proof using.
 Qed.
 
 
-Definition counter_WF_spec (l: loc): WaitFreeSpec (incr l) := {|
+Definition counter_WF_spec (l: loc): WaitFreeSpec trillium.bi.weakestpre.NotStuck (incr l) := {|
   wfs_init_mod Σ _ _ := counter_wfree_init_inv l;
   wfs_spec := @counter_wfree_spec l;
   wfs_safety_spec Σ _ _ := counter_safety_spec l;
