lawyer/nonblocking/examples/counter_adequacy.v
@@ -3,7 +3,7 @@ From lawyer.nonblocking Require Import counter wfree_adequacy wfree_traces.
 
 Theorem counter_is_wait_free
   (l0: loc := Loc 0)
-  : wait_free (incr l0) (counter_is_init_st l0).
+  : wait_free (incr l0) (counter_is_init_st l0) NotStuck.
 Proof using.
   eapply (wfree_is_wait_free _ (counter_WF_spec l0)).
   eauto. 
